\section{Transformada de Fourier}

\begin{frame}
	\frametitle{
		\secname~(\citeauthor[p.~637]{salgado_classical_2022})
	} % \citetitle

	\begin{equation*}
		\widehat{v}\left(\xi\right)=
		\mathcal{F}\left[v\right]\left(\xi\right)=
		\int_{\mathbb{R}^{d}}
		\exp\left(-ix\xi\right)
		v\left(x\right)\dl x
	\end{equation*}

	\begin{equation*}
		\left(
		\widehat{
			\difcp{u}{t}-
			\alpha^{2}\difc.L.{u}{}
		}
		\right)
		\left(k,t\right)=
		\widehat{\left(\difcp{u}{t}\right)}
		\left(k,t\right)-
		\widehat{\alpha^{2}\difc.L.{u}{}}
		\left(k,t\right)
		=\widehat{0}=
		0
	\end{equation*}

	\begin{equation*}
		\widehat{\left(\difcp{u}{t}\right)}
		\left(k,t\right)=
		\int_{-\infty}^{\infty}
		\difcp{u}{t}
		\left(x,t\right)
		\exp\left(-ikx\right)
		\dl x=
		\difcp{}{t} % TODO:
		\left(
		\int_{-\infty}^{\infty}
		u
		\left(x,t\right)
		\right)
		\exp\left(-ikx\right)
		\dl x=
		\difcp{\widehat{u}\left(k,t\right)}{t}=
		\difcp{\widehat{u}}{t}=
	\end{equation*}
\end{frame}


\begin{frame}
	\begin{equation*}
		\widehat{\difcp[2]{u}{x}}
		\left(k,t\right)=
		\left(ik\right)^{2}
		\widehat{u}
		\left(k,t\right)=
		-k^{2}
		\widehat{u}
		\left(k,t\right)=
	\end{equation*}

	Para cada $k$, $f\left(t\right)\coloneqq\widehat{u}\left(k,t\right)$

	\begin{equation*}
		F\left(x\right)=
		\dfrac{1}{\sqrt{4\pi t}}
		\exp\left(-\dfrac{x^{2}}{4t}\right)
	\end{equation*}

	\begin{equation*}
		u\left(x,t\right)=
		\dfrac{1}{\sqrt{4\pi\alpha t}}
		\int_{-\infty}^{\infty}
		\exp\left(-\dfrac{{\left(x-y\right)}^{2}}{4\alpha t}\right)
		g\left(y\right)\dl y
	\end{equation*}

	\begin{proof}
		\begin{equation*}
			u\left(x,t\right)-
			u_{0}\left(x_{0}\right)=
			\dfrac{1}{{\left(4\pi t\right)}^{d/2}}
			\int_{\mathbb{R}^{d}}
			\exp\left(-\dfrac{{\left\|x-y\right\|}^{2}_{2}}{4t}\right)
			u_{0}\left(y\right)\dl y-
			u_{0}\left(x_{0}\right)
		\end{equation*}
	\end{proof}
\end{frame}
